wip

lib/hst/Hacl.UInt128.fst
@@ -21,13 +21,6 @@ val add: a:t -> b:t -> Pure t
 let add a b =
   Mk (add (a.v) (b.v))
 
-(* val add_underspec: a:t -> b:t -> Pure t *)
-(*   (requires True) *)
-(*   (ensures (fun c -> *)
-(*     UInt.size (v a + v b) n ==> v a + v b = v c)) *)
-(* let add_underspec a b = *)
-(*   Mk (add_underspec (a.v) (b.v)) *)
-
 val add_mod: a:t -> b:t -> Pure t
   (requires True)
   (ensures (fun c -> (v a + v b) % pow2 n = v c))
@@ -41,13 +34,6 @@ val sub: a:t -> b:t -> Pure t
 let sub a b =
   Mk (sub (a.v) (b.v))
 
-(* val sub_underspec: a:t -> b:t -> Pure t *)
-(*   (requires True) *)
-(*   (ensures (fun c -> *)
-(*     UInt.size (v a - v b) n ==> v a - v b = v c)) *)
-(* let sub_underspec a b = *)
-(*   Mk (sub_underspec (a.v) (b.v)) *)
-
 val sub_mod: a:t -> b:t -> Pure t
   (requires True)
   (ensures (fun c -> (v a - v b) % pow2 n = v c))
@@ -55,45 +41,17 @@ let sub_mod a b =
   Mk (sub_mod (a.v) (b.v))
 
 (* Multiplication primitives *)
-(* val mul: a:t -> b:t -> Pure t *)
-(*   (requires (UInt.size (v a * v b) n)) *)
-(*   (ensures (fun c -> v a * v b = v c)) *)
-(* let mul a b = *)
-(*   Mk (mul (a.v) (b.v)) *)
+val mul: a:t -> b:t -> Pure t
+  (requires (UInt.size (v a * v b) n))
+  (ensures (fun c -> v a * v b = v c))
+let mul a b =
+  Mk (mul (a.v) (b.v))
 
-(* val mul_underspec: a:t -> b:t -> Pure t *)
-(*   (requires True) *)
-(*   (ensures (fun c -> *)
-(*     UInt.size (v a * v b) n ==> v a * v b = v c)) *)
-(* let mul_underspec a b = *)
-(*   Mk (mul_underspec (a.v) (b.v)) *)
-
-(* val mul_mod: a:t -> b:t -> Pure t *)
-(*   (requires True) *)
-(*   (ensures (fun c -> (v a * v b) % pow2 n = v c)) *)
-(* let mul_mod a b = *)
-(*   Mk (mul_mod (a.v) (b.v)) *)
-
-(* Division primitives *)
-(* val div: a:t -> b:t{v b <> 0} -> Pure t *)
-(*   (requires (UInt.size (v a / v b) n)) *)
-(*   (ensures (fun c -> v b <> 0 ==> v a / v b = v c)) *)
-(* let div a b = *)
-(*   Mk (div (a.v) (b.v)) *)
-
-(* val div_underspec: a:t -> b:t{v b <> 0} -> Pure t *)
-(*   (requires True) *)
-(*   (ensures (fun c -> *)
-(*     (v b <> 0 /\ UInt.size (v a / v b) n) ==> v a / v b = v c)) *)
-(* let div_underspec a b = *)
-(*   Mk (div_underspec (a.v) (b.v)) *)
-
-(* Modulo primitives *)
-(* val rem: a:t -> b:t{v b <> 0} -> Pure t *)
-(*   (requires True) *)
-(*   (ensures (fun c -> *)
-(*     v a - ((v a / v b) * v b) = v c)) *)
-(* let rem a b = Mk (rem (a.v) (b.v)) *)
+val mul_mod: a:t -> b:t -> Pure t
+  (requires True)
+  (ensures (fun c -> (v a * v b) % pow2 n = v c))
+let mul_mod a b =
+  Mk (mul_mod (a.v) (b.v))
 
 (* Bitwise operators *)
 val logand: t -> t -> Tot t
@@ -105,10 +63,10 @@ let logor a b = Mk (logor (a.v) (b.v))
 val lognot: t -> Tot t
 let lognot a = Mk (lognot (a.v))
 
-(* val uint_to_t: x:(UInt.uint_t n) -> Pure t *)
-(*   (requires True) *)
-(*   (ensures (fun y -> v y = x)) *)
-(* let uint_to_t x = Mk (uint_to_t x) *)
+val uint_to_t: x:(UInt.uint_t n) -> Pure t
+  (requires True)
+  (ensures (fun y -> v y = x))
+let uint_to_t x = Mk (uint_to_t x)
 
 (* Shift operators *)
 val shift_right: a:t -> s:FStar.UInt32.t -> Pure t
@@ -129,16 +87,11 @@ assume val lte_mask: a:t -> b:t -> Tot (c:t{(v a <= v b ==> v c = pow2 n - 1) /\
 
 (* Infix notations *)
 let op_Plus_Hat = add
-(* let op_Plus_Question_Hat = add_underspec *)
 let op_Plus_Percent_Hat = add_mod
 let op_Subtraction_Hat = sub
-(* let op_Subtraction_Question_Hat = sub_underspec *)
 let op_Subtraction_Percent_Hat = sub_mod
-(* let op_Star_Hat = mul *)
-(* let op_Star_Question_Hat = mul_underspec *)
-(* let op_Star_Percent_Hat = mul_mod *)
-(* let op_Slash_Hat = div *)
-(* let op_Percent_Hat = rem *)
+let op_Star_Hat = mul
+let op_Star_Percent_Hat = mul_mod
 let op_Hat_Hat = logxor
 let op_Amp_Hat = logand
 let op_Bar_Hat = logor
