lib/hst/kremlin/Hacl.UInt64.fst
@@ -14,129 +14,88 @@ type t = U.t
 
 let v (x:t) : GTot (FStar.UInt.uint_t n) = U.v x
 
-val add: a:t -> b:t -> Pure t
-  (requires (UInt.size (v a + v b) n))
-  (ensures (fun c -> v a + v b = v c))
-let add a b = add a b
+inline_for_extraction val add: a:t -> b:t{UInt.size (v a + v b) n} -> Tot (c:t{v a + v b = v c})
+inline_for_extraction let add a b = add a b
 
-(* val add_underspec: a:t -> b:t -> Pure t *)
-(*   (requires True) *)
-(*   (ensures (fun c -> *)
-(*     UInt.size (v a + v b) n ==> v a + v b = v c)) *)
-(* let add_underspec a b = add_underspec a b *)
-
-val add_mod: a:t -> b:t -> Pure t
-  (requires True)
-  (ensures (fun c -> (v a + v b) % pow2 n = v c))
-let add_mod a b = add_mod a b
+inline_for_extraction val add_mod: a:t -> b:t -> Tot (c:t{(v a + v b) % pow2 n = v c})
+inline_for_extraction let add_mod a b = add_mod a b
 
 (* Subtraction primitives *)
-val sub: a:t -> b:t -> Pure t
-  (requires (UInt.size (v a - v b) n))
-  (ensures (fun c -> v a - v b = v c))
-let sub a b = sub a b
+inline_for_extraction val sub: a:t -> b:t{(UInt.size (v a - v b) n)} -> Tot (c:t{v a - v b = v c})
+inline_for_extraction let sub a b = sub a b
 
-(* val sub_underspec: a:t -> b:t -> Pure t *)
-(*   (requires True) *)
-(*   (ensures (fun c -> *)
-(*     UInt.size (v a - v b) n ==> v a - v b = v c)) *)
-(* let sub_underspec a b = sub_underspec a b *)
-
-val sub_mod: a:t -> b:t -> Pure t
-  (requires True)
-  (ensures (fun c -> (v a - v b) % pow2 n = v c))
-let sub_mod a b = sub_mod a b
+inline_for_extraction val sub_mod: a:t -> b:t -> Tot (c:t{(v a - v b) % pow2 n = v c})
+inline_for_extraction let sub_mod a b = sub_mod a b
 
 (* Multiplication primitives *)
-val mul: a:t -> b:t -> Pure t
-  (requires (UInt.size (v a * v b) n))
-  (ensures (fun c -> v a * v b = v c))
-let mul a b = mul a b
+inline_for_extraction val mul: a:t -> b:t{UInt.size (v a * v b) n} -> Tot (c:t{v a * v b = v c})
+inline_for_extraction let mul a b = mul a b
 
-(* val mul_underspec: a:t -> b:t -> Pure t *)
-(*   (requires True) *)
-(*   (ensures (fun c -> *)
-(*     UInt.size (v a * v b) n ==> v a * v b = v c)) *)
-(* let mul_underspec a b = mul_underspec a b *)
-
-val mul_mod: a:t -> b:t -> Pure t
-  (requires True)
-  (ensures (fun c -> (v a * v b) % pow2 n = v c)) 
-let mul_mod a b = mul_mod a b
-
-(* Division primitives *)
-val div: a:t -> b:t{v b <> 0} -> Pure t
-  (requires (UInt.size (v a / v b) n))
-  (ensures (fun c -> v b <> 0 ==> v a / v b = v c))
-let div a b = div a b
-
-(* val div_underspec: a:t -> b:t{v b <> 0} -> Pure t *)
-(*   (requires True) *)
-(*   (ensures (fun c -> *)
-(*     (v b <> 0 /\ UInt.size (v a / v b) n) ==> v a / v b = v c)) *)
-(* let div_underspec a b = div_underspec a b *)
-
-(* Modulo primitives *)
-val rem: a:t -> b:t{v b <> 0} -> Pure t
-  (requires True)
-  (ensures (fun c ->
-    v a - ((v a / v b) * v b) = v c))
-let rem a b = rem a b
+inline_for_extraction val mul_mod: a:t -> b:t -> Tot (c:t{(v a * v b) % pow2 n = v c})
+inline_for_extraction let mul_mod a b = mul_mod a b
 
 (* Bitwise operators *)
-val logand: t -> t -> Tot t
-let logand a b = logand a b
-val logxor: t -> t -> Tot t
-let logxor a b = logxor a b
-val logor: t -> t -> Tot t
-let logor a b = logor a b
-val lognot: t -> Tot t
-let lognot a = lognot a
-
-(* val uint_to_t: x:(UInt.uint_t n) -> Pure t *)
-(*   (requires True) *)
-(*   (ensures (fun y -> v y = x)) *)
-(* let uint_to_t x = uint_to_t x *)
+inline_for_extraction val logand: t -> t -> Tot t
+inline_for_extraction let logand a b = logand a b
+inline_for_extraction val logxor: t -> t -> Tot t
+inline_for_extraction let logxor a b = logxor a b
+inline_for_extraction val logor: t -> t -> Tot t
+inline_for_extraction let logor a b = logor a b
+inline_for_extraction val lognot: t -> Tot t
+inline_for_extraction let lognot a = lognot a
 
 (* Shift operators *)
-val shift_right: a:t -> s:FStar.UInt32.t -> Pure t
-  (requires True)
-  (ensures (fun c -> FStar.UInt32.v s < n ==> v c = (v a / (pow2 (FStar.UInt32.v s)))))
-let shift_right a s = shift_right a s
+inline_for_extraction val shift_right: a:t -> s:FStar.UInt32.t -> Tot (c:t{FStar.UInt32.v s < n ==> v c = (v a / (pow2 (FStar.UInt32.v s)))})
+inline_for_extraction let shift_right a s = shift_right a s
 
-val shift_left: a:t -> s:FStar.UInt32.t -> Pure t
-  (requires True)
-  (ensures (fun c -> FStar.UInt32.v s < n ==> v c = ((v a * pow2 (FStar.UInt32.v s)) % pow2 n)))
-let shift_left a s = shift_left a s
+inline_for_extraction val shift_left: a:t -> s:FStar.UInt32.t -> Tot (c:t{FStar.UInt32.v s < n ==> v c = ((v a * pow2 (FStar.UInt32.v s)) % pow2 n)})
+inline_for_extraction let shift_left a s = shift_left a s
 
-val eq_mask: a:t -> b:t -> Tot (c:t{(v a = v b ==> v c = pow2 n - 1) /\ (v a <> v b ==> v c = 0)})
-let eq_mask a b = eq_mask a b
-val gte_mask: a:t -> b:t -> Tot (c:t{(v a >= v b ==> v c = pow2 n - 1) /\ (v a < v b ==> v c = 0)})
-let gte_mask a b = gte_mask a b
-val gt_mask: a:t -> b:t -> Tot (c:t{(v a > v b ==> v c = pow2 n - 1) /\ (v a <= v b ==> v c = 0)})
-let gt_mask a b = lognot (gte_mask b a)
-val lt_mask: a:t -> b:t -> Tot (c:t{(v a < v b ==> v c = pow2 n - 1) /\ (v a >= v b ==> v c = 0)})
-let lt_mask a b = lognot (gte_mask a b)
-val lte_mask: a:t -> b:t -> Tot (c:t{(v a <= v b ==> v c = pow2 n - 1) /\ (v a > v b ==> v c = 0)})
-let lte_mask a b = lognot (gt_mask a b)
+inline_for_extraction val eq_mask: a:t -> b:t -> Tot (c:t{(v a = v b ==> v c = pow2 n - 1) /\ (v a <> v b ==> v c = 0)})
+inline_for_extraction let eq_mask a b = eq_mask a b
+inline_for_extraction val gte_mask: a:t -> b:t -> Tot (c:t{(v a >= v b ==> v c = pow2 n - 1) /\ (v a < v b ==> v c = 0)})
+inline_for_extraction let gte_mask a b = gte_mask a b
+inline_for_extraction val gt_mask: a:t -> b:t -> Tot (c:t{(v a > v b ==> v c = pow2 n - 1) /\ (v a <= v b ==> v c = 0)})
+inline_for_extraction let gt_mask a b = lognot (gte_mask b a)
+inline_for_extraction val lt_mask: a:t -> b:t -> Tot (c:t{(v a < v b ==> v c = pow2 n - 1) /\ (v a >= v b ==> v c = 0)})
+inline_for_extraction let lt_mask a b = lognot (gte_mask a b)
+inline_for_extraction val lte_mask: a:t -> b:t -> Tot (c:t{(v a <= v b ==> v c = pow2 n - 1) /\ (v a > v b ==> v c = 0)})
+inline_for_extraction let lte_mask a b = lognot (gt_mask a b)
+
 
 (* Infix notations *)
-let op_Plus_Hat = add
-(* let op_Plus_Question_Hat = add_underspec *)
-let op_Plus_Percent_Hat = add_mod
-let op_Subtraction_Hat = sub
-(* let op_Subtraction_Question_Hat = sub_underspec *)
-let op_Subtraction_Percent_Hat = sub_mod
-let op_Star_Hat = mul
-(* let op_Star_Question_Hat = mul_underspec *)
-let op_Star_Percent_Hat = mul_mod
-let op_Slash_Hat = div
-let op_Percent_Hat = rem
-let op_Hat_Hat = logxor
-let op_Amp_Hat = logand
-let op_Bar_Hat = logor
-let op_Less_Less_Hat = shift_left
-let op_Greater_Greater_Hat = shift_right
+
+inline_for_extraction val op_Plus_Hat: a:t -> b:t{UInt.size (v a + v b) n} -> Tot (c:t{v a + v b = v c})
+inline_for_extraction let op_Plus_Hat a b = add a b
+
+inline_for_extraction val op_Plus_Percent_Hat: a:t -> b:t -> Tot (c:t{(v a + v b) % pow2 n = v c})
+inline_for_extraction let op_Plus_Percent_Hat a b = add_mod a b
+
+inline_for_extraction val op_Subtraction_Hat: a:t -> b:t{(UInt.size (v a - v b) n)} -> Tot (c:t{v a - v b = v c})
+inline_for_extraction let op_Subtraction_Hat a b = sub a b
+
+inline_for_extraction val op_Subtraction_Percent_Hat: a:t -> b:t -> Tot (c:t{(v a - v b) % pow2 n = v c})
+inline_for_extraction let op_Subtraction_Percent_Hat a b = sub_mod a b
+
+inline_for_extraction val op_Star_Hat: a:t -> b:t{UInt.size (v a * v b) n} -> Tot (c:t{v a * v b = v c})
+inline_for_extraction let op_Star_Hat a b = mul a b
+
+inline_for_extraction val op_Star_Percent_Hat: a:t -> b:t -> Tot (c:t{(v a * v b) % pow2 n = v c})
+inline_for_extraction let op_Star_Percent_Hat a b = mul_mod a b
+
+inline_for_extraction val op_Amp_Hat: t -> t -> Tot t
+inline_for_extraction let op_Amp_Hat a b = logand a b
+inline_for_extraction val op_Hat_Hat: t -> t -> Tot t
+inline_for_extraction let op_Hat_Hat a b = logxor a b
+inline_for_extraction val op_Bar_Hat: t -> t -> Tot t
+inline_for_extraction let op_Bar_Hat a b = logor a b
+
+(* Shift operators *)
+inline_for_extraction val op_Greater_Greater_Hat: a:t -> s:FStar.UInt32.t -> Tot (c:t{FStar.UInt32.v s < n ==> v c = (v a / (pow2 (FStar.UInt32.v s)))})
+inline_for_extraction let op_Greater_Greater_Hat a s = shift_right a s
+
+inline_for_extraction val op_Less_Less_Hat: a:t -> s:FStar.UInt32.t -> Tot (c:t{FStar.UInt32.v s < n ==> v c = ((v a * pow2 (FStar.UInt32.v s)) % pow2 n)})
+inline_for_extraction let op_Less_Less_Hat a s = shift_left a s
 
 (* To input / output constants *)
 assume val of_string: string -> Tot t
